\documentclass[UTF8,a4paper]{ctexart}
\usepackage[utf8]{inputenc}
\usepackage{amsmath}
\usepackage{pdfpages}
\usepackage{graphicx}
\usepackage{wrapfig}
\usepackage{listings}
\title{模式识别作业1}
\author{张蔚桐\ 2015011493\ 自55}
\begin {document}
\maketitle
\section{}
根据线性回归方程可以得到$$\begin{aligned}
\hat{y}=\hat{\theta_0}+\hat{\theta_1}x \\ 
\hat{\theta_0}=\bar{y}-\hat{\theta_1}\bar{x} \\
\hat{\theta_1}=\frac{E((y-E(y))(x-E(x)))}{D(x)}\\
\end{aligned}$$其中$D(x),E(x)$分别为样本的方差和期望,
因此可以得到$$\begin{aligned}
R^2=\frac{E((\bar{y}-\hat{y})^2)}{D(y)} \\
r^2=\frac{E((y-E(y))(x-E(x)))}{D(x)D(y)} \end{aligned} $$
欲证$R^2=r^2$即证明$$E((\bar{y}-\hat{y})^2)=\frac{E((y-E(y))(x-E(x)))}{D(x)}$$
左侧$$\begin{aligned}=E^2(y)-2E(y)E(\hat{\theta_0}+\hat{\theta_1}x) - E((\hat{\theta_0}+\hat{\theta_1}x)^2)\\ =E^2(y)-2E(y)E(\bar{y}+\hat{\theta_1}(x-\bar{x})+E((\bar{y}+\hat{\theta_1}(x-\bar{x})^2)
\end{aligned}$$

\end{document}